Add files via upload

new_model/SPI_rxScript.sml
@@ -15,12 +15,15 @@ rx := spi.rx with state := rx_receive_data |>`
 
 (* SPI controller operation that indicates the hardware receives data(a word)
  * from the slave over the wire, Slave shift reg -> Master SPI shift reg.
- * rx_receive_data_op: environment -> spi_state -> spi_state
+ * rx_receive_data_op: spi_state -> spi_state -> word8 option -> spi_state
  *)
 val rx_receive_data_op_def = Define `
-rx_receive_data_op (env:environment) (spi:spi_state) =
-spi with <| SHIFT_REG := env.SHIFT_REG; (* a word is received over the wire *)
-rx := spi.rx with state := rx_update_RX0 |>`
+rx_receive_data_op (spi:spi_state) (spi':spi_state) (data: word8 option) =
+if (spi'.tx.state = tx_trans_done) /\ (spi.rx.state = rx_receive_data) 
+/\ (spi.regs.CH0STAT.RXS = 0w) /\ (data <> NONE) then 
+spi with <| RX_SHIFT_REG := THE data; (* a word is received over the wire *)
+rx := spi.rx with state := rx_update_RX0 |>
+else spi`
 
 (* SPI controller operation when the received word is transferred
  * from the shift register to the RX0 register, shift reg -> RX0.
@@ -30,7 +33,7 @@ val rx_update_RX0_op_def = Define `
 rx_update_RX0_op (spi:spi_state) =
 spi with <| regs := spi.regs with
 (* a received word is transferred from shift register to RX0 *)
-<|RX0 := w2w spi.SHIFT_REG;
+<|RX0 := w2w spi.RX_SHIFT_REG;
 CH0STAT := spi.regs.CH0STAT with RXS := 1w |>;
 rx := spi.rx with state := rx_data_ready |>`
 
@@ -47,12 +50,12 @@ else spi with err := T`
  * spi_rx_operations: spi_state -> spi_state
  *)
 val spi_rx_operations_def = Define `
-spi_rx_operations (env:environment) (spi: spi_state) =
+spi_rx_operations (spi:spi_state) =
 case spi.rx.state of
 | rx_idle => spi with err := T
 | rx_conf_ready => spi with err := T
 | rx_channel_enabled => rx_channel_enabled_op spi
-| rx_receive_data => rx_receive_data_op env spi
+| rx_receive_data => spi with err := T
 | rx_update_RX0 => rx_update_RX0_op spi 
 | rx_data_ready => spi with err := T
 | rx_receive_check => rx_receive_check_op spi
