new_model/SPI_relationScript.sml
@@ -1,0 +1,91 @@
+open HolKernel bossLib boolLib Parse;
+open wordsTheory wordsLib;
+open SPI_stateTheory write_SPIregsTheory read_SPIregsTheory SPI_initTheory SPI_txTheory SPI_rxTheory;
+
+val _ = new_theory "SPI_relation";
+
+(* tr: (state) transition *)
+(* Some functions return specific datatypes *)
+val read_SPI_regs_state_def = Define `
+read_SPI_regs_state (env:environment) (pa:word32) (spi:spi_state) =
+let (spi', v) = read_SPI_regs env pa spi in spi'`
+
+val read_SPI_regs_value_def = Define `
+read_SPI_regs_value (env:environment) (pa:word32) (spi:spi_state) =
+let (spi', v) = read_SPI_regs env pa spi in v`
+
+val tx_trans_done_op_state_def = Define `
+tx_trans_done_op_state (spi:spi_state) (spi':spi_state) =
+let (spi_new, v_option) = tx_trans_done_op spi spi' in spi_new`
+
+val tx_trans_done_op_value_def = Define `
+x_trans_done_op_value (spi:spi_state) (spi':spi_state) =
+let (spi_new, v_option) = tx_trans_done_op spi spi' in v_option`
+
+(* relation for spi transition (an SPI device).
+ * Here spi' is another spi device.
+ *)
+val (spi_tr_rules, spi_tr_ind, spi_tr_cases) = Hol_reln `
+(!(spi:spi_state). T ==> spi_tr spi (Update a v) (write_SPI_regs a v spi)) /\
+(!(spi:spi_state). T ==> spi_tr spi (Return a (read_SPI_regs_value env a spi)) (read_SPI_regs_state env a spi)) /\
+(!(spi:spi_state). (env.scheduler = Initialize) /\ (INIT_ENABLE spi) ==>
+spi_tr spi tau (spi_init_operations spi)) /\
+(!(spi:spi_state). (env.scheduler = Transmit) /\ (TX_ENABLE spi) ==>
+spi_tr spi tau (spi_tx_operations spi)) /\
+(!(spi:spi_state). (env.scheduler = Receive) /\ (RX_ENABLE spi) ==>
+spi_tr spi tau (spi_rx_operations spi)) /\
+(!(spi:spi_state) (spi':spi_state). (spi.tx.state = tx_trans_done) ==> 
+spi_tr spi (TX (tx_trans_done_op_value spi spi')) (tx_trans_done_op_state spi spi')) /\
+(!(spi:spi_state) (spi':spi_state). (spi.rx.state = rx_receive_data) ==> 
+spi_tr spi (RX data) (rx_receive_data_op spi spi' data))`
+
+(* relation for local transition (an SPI device and a CPU)
+ * CPU's datatype could be arm_state or the driver's datatype we defined later.
+ *)
+val (local_tr_rules, local_tr_ind, local_tr_cases) = Hol_reln `
+(!(cpu:'a) (spi:spi_state).
+cpu_tr cpu tau cpu' ==> local_tr (cpu, spi) tau (cpu', spi)) /\
+(!(cpu:'a) (spi:spi_state).
+spi_tr spi tau spi' ==> local_tr (cpu, spi) tau (cpu, spi')) /\
+(!(cpu:'a) (spi:spi_state).
+(cpu_tr cpu (Write a v) cpu') /\
+(spi_tr spi (Update a v) spi') ==>
+local_tr (cpu, spi) tau (cpu', spi')) /\
+(!(cpu:'a) (spi:spi_state).
+(cpu_tr cpu (Read a) cpu') /\
+(spi_tr spi (Return a v) spi') ==>
+local_tr (cpu, spi) tau (cpu', spi')) /\
+(!(cpu:'a) (spi:spi_state).
+spi_tr spi (TX data) spi' ==> local_tr (cpu, spi) (TX data) (cpu, spi')) /\
+(!(cpu:'a) (spi:spi_state).
+spi_tr spi (RX data) spi' ==> local_tr (cpu, spi) (RX data) (cpu, spi'))`
+
+(* relation for global transition (two SPI devices and two CPUs) *)
+val (gloabl_tr_rules, global_tr_ind, global_tr_cases) = Hol_reln `
+(!(cpu1:'a) (spi1:spi_state) (cpu2:'a) (spi2:spi_state). 
+local_tr (cpu1, spi1) tau (cpu1', spi1') ==>
+global_tr (cpu1, spi1, cpu2, spi2) (cpu1', spi1', cpu2, spi2)) /\
+(!(cpu1:'a) (spi1:spi_state) (cpu2:'a) (spi2:spi_state). 
+local_tr (cpu2, spi2) tau (cpu2', spi2') ==>
+global_tr (cpu1, spi1, cpu2, spi2) (cpu1, spi1, cpu2', spi2')) /\
+(!(cpu1:'a) (spi1:spi_state) (cpu2:'a) (spi2:spi_state). 
+(local_tr (cpu1, spi1) (TX data) (cpu1', spi1')) /\
+(local_tr (cpu2, spi2) (RX data) (cpu2', spi2')) ==>
+global_tr (cpu1, spi1, cpu2, spi2) (cpu1', spi1', cpu2', spi2')) /\
+(!(cpu1:'a) (spi1:spi_state) (cpu2:'a) (spi2:spi_state). 
+(local_tr (cpu1, spi1) (RX data) (cpu1', spi1')) /\
+(local_tr (cpu2, spi2) (TX data) (cpu2', spi2')) ==>
+global_tr (cpu1, spi1, cpu2, spi2) (cpu1', spi1', cpu2', spi2'))`
+
+
+val SPI_rx_data = store_thm("SPI_rx_data",
+``!spi1 spi1' spi2 data. 
+(data <> NONE) /\ (spi1.rx.state = rx_receive_data) /\ (spi1.regs.CH0STAT.RXS = 0w) /\
+(spi1' = rx_receive_data_op spi1 spi2 data) /\ (spi2.tx.state = tx_trans_done) /\
+(spi_tr spi1 (RX data) spi1') 
+==> (spi1'.RX_SHIFT_REG = THE data)``,
+REPEAT STRIP_TAC >>
+FULL_SIMP_TAC std_ss [spi_tr_cases] >>
+RW_TAC std_ss [rx_receive_data_op_def]);
+
+val _ = export_theory();
