new_model/SPI_txScript.sml
@@ -13,29 +13,30 @@ spi with <|regs := spi.regs with CH0STAT := spi.regs.CH0STAT
 with TXS := 1w; (* TXS is set to 1 when enable channel 0 *)
 tx := spi.tx with state := tx_ready_for_trans |>`
 
-(* SPI controller's operation if it starts to transmit data. (TX0 -> shift Reg)
+(* SPI controller's operation if it starts to transmit data. 
+ * TX0 -> TX_SHIFT_REG, SPI internal data transition.
  * tx_trans_data_op: spi_state -> spi_state 
  *)
 val tx_trans_data_op_def = Define `
 tx_trans_data_op (spi:spi_state) =
-spi with <| (* Data is transferred from TX0 to the shift register (the wire) *)
-SHIFT_REG := w2w spi.regs.TX0;
+spi with <| TX_SHIFT_REG := w2w spi.regs.TX0;
 regs := spi.regs with CH0STAT := spi.regs.CH0STAT
 with <|EOT := 0w; TXS := 1w|>; (* EOT bit is cleared, TXS bit is set*)  
 tx := spi.tx with state := tx_trans_done |>`
 
-(* SPI controller's operation when the data 
- * is transferred to the slave over the wire. (shift Reg -> slave shift Reg)
- * tx_trans_done_op: spi_state -> spi_state
+(* SPI controller's operation when the data is transferred to another SPI device.
+ * It's not the SPI internal operation, but depends on SPI slave's state.
+ * master TX_SHIFT_REG -> slave RX_SHIFT_REG, shows the interactions between master and slave.
+ * tx_trans_done_op: spi_state -> spi_state -> spi_state * word8 option
  *)
-(* update the env with SHIFT_REG := spi.SHIFT_REG *)
 val tx_trans_done_op_def = Define `
-tx_trans_done_op (spi:spi_state) =
-spi with <|regs := spi.regs with CH0STAT := spi.regs.CH0STAT
-(* An SPI word is transferred from the shift register to the slave *)
-with EOT := 1w;
-tx := spi.tx with state := tx_trans_check |>`
-
+tx_trans_done_op (spi:spi_state) (spi':spi_state) =
+if (spi.tx.state = tx_trans_done) /\ (spi'.rx.state = rx_receive_data) /\ (spi'.regs.CH0STAT.RXS = 0w) then
+(spi with <|regs := spi.regs with CH0STAT := spi.regs.CH0STAT
+(* An SPI word is transferred from the rx shift register to the slave *)
+with EOT := 1w|>,
+SOME spi.TX_SHIFT_REG)
+else (spi, NONE)`
 
 (* SPI controller's operation after EOT bit is set to 1.
  * tx_trans_check_op: spi_state -> spi_state
@@ -47,7 +48,7 @@ spi with tx := spi.tx with state := tx_ready_for_trans
 else spi with err := T`
 
 (* This function indicates SPI controller's internal operations for tx automaton.
- * spi_tx_operations: spi_state -> spi_state 
+ * spi_tx_operations: spi_state -> spi_state -> spi_state * word8 option
  *)
 val spi_tx_operations_def = Define `
 spi_tx_operations (spi:spi_state) =
@@ -57,9 +58,8 @@ case spi.tx.state of
   | tx_channel_enabled => tx_channel_enabled_op spi 
   | tx_ready_for_trans => spi with err := T
   | tx_trans_data => tx_trans_data_op spi
-  | tx_trans_done => tx_trans_done_op spi
+  | tx_trans_done => spi with err := T
   | tx_trans_check => tx_trans_check_op spi
   | tx_channel_disabled => spi with err := T`
-
 
 val _ = export_theory();
